src/linear/implementation/DoublyLinkedListWithLast.dfy
@@ -1,0 +1,151 @@
+include "../../../src/linear/implementation/DoublyLinkedList.dfy"
+
+class DoublyLinkedListWithLast {
+  var list: DoublyLinkedList;
+  var last: Node?;
+
+  predicate Valid()
+    reads this, list, list.spine
+  {
+    && list.Valid()
+    && (if last == null then
+        list.head == null
+      else
+        last in list.Repr() && last.next == null
+      )
+  }
+
+  function Repr(): set<object>
+    reads this, list, list.spine
+  {
+    list.Repr()
+  }
+
+  function Model(): seq<A>
+    reads this, list, list.spine
+    requires Valid()
+  {
+    list.Model()
+  }
+
+  constructor()
+    ensures Valid()
+  {
+    list := new DoublyLinkedList();
+    last := null;
+  }
+
+  // O(1)
+  method PushFront(x: A)
+    modifies this, list, Repr()
+    requires Valid()
+    ensures Valid()
+    ensures Model() == [x] + old(Model())
+    ensures Repr() > old(Repr())
+    ensures fresh(Repr() - old(Repr()))
+  {
+    var ohead := list.head;
+    { // GHOST
+      if ohead != null {
+        list.LastHasLastIndex(last);
+      }
+    }
+    list.PushFront(x);
+    if ohead == null {
+      last := list.head;
+    }
+  }
+
+  // O(1)
+  method PopFront() returns (x: A)
+    modifies this, list, Repr()
+    requires Valid()
+    requires Model() != []
+    ensures Valid()
+    ensures [x] + Model() == old(Model())
+    ensures Repr() < old(Repr())
+  {
+    { // GHOST
+      if list.head != null {
+        list.LastHasLastIndex(last);
+      }
+    }
+    if list.head == last {
+      last := null;
+    }
+    { // GHOST
+      if list.head.next != null {
+        assert list.head == list.spine[0];
+        assert list.head.next == list.spine[1];
+        assert list.head.next in Repr();
+      }
+    }
+    x := list.PopFront();
+  }
+
+  // O(1)
+  method PushBack(x: A)
+    modifies this, list, Repr()
+    requires Valid()
+    ensures Valid()
+    ensures Model() == old(Model()) + [x]
+    ensures Repr() > old(Repr())
+    ensures fresh(Repr() - old(Repr()))
+  {
+    if last == null {
+      assert Model() == [];
+      list.PushFront(x);
+      last := list.head;
+    } else {
+      { // GHOST
+        list.LastHasLastIndex(last);
+        list.ModelRelationWithSpine();
+      }
+      list.Insert(last, x);
+      last := last.next;
+      assert last != null;
+      assert Valid();
+    }
+  }
+
+  // O(1)
+  method PopBack() returns (x: A)
+    modifies this, list, list.Repr()
+    requires Valid()
+    requires Model() != []
+    ensures Valid()
+    ensures Model() + [x] == old(Model())
+    ensures Repr() < old(Repr())
+  {
+    if list.head == last {
+      assert list.head.next == null;
+      list.HeadNextNullImpliesSingleton();
+      assert list.spine == [list.head];
+      calc == {
+        list.Model();
+        list.ModelAux(list.spine);
+        [list.head.data];
+      }
+      x := list.head.data;
+      list.head := null;
+      /*GHOST*/ list.spine := [];
+      last := null;
+      assert old(list.Model()) == [x];
+      assert Model() + [x] == old(Model());
+      assert Repr() < old(Repr());
+    } else {
+      x := last.data;
+      var prev := last.prev;
+      { // GHOST
+        list.ModelRelationWithSpine();
+        list.LastHasLastIndex(last);
+        assert last == list.spine[|list.spine|-1];
+        assert last.prev == list.spine[|list.spine|-2];
+        assert prev in Repr();
+        assert last in Repr();
+      }
+      list.RemoveNext(prev);
+      last := prev;
+    }
+  }
+}
